case_study/RiscvPmp/Machine.v
@@ -193,6 +193,7 @@ Module Import RiscvPmpProgram <: Program RiscvPmpBase.
   | close_gprs            : Lem ctx.nil
   | open_pmp_entries      : Lem ctx.nil
   | close_pmp_entries     : Lem ctx.nil
+  | update_pmp_entries    : Lem ctx.nil
   | extract_pmp_ptsto     : Lem [paddr :: ty_xlenbits]
   | return_pmp_ptsto      : Lem [paddr :: ty_xlenbits]
   .
@@ -545,9 +546,10 @@ Module Import RiscvPmpProgram <: Program RiscvPmpBase.
     call tick_pc.
 
   Definition fun_init_sys : Stm ctx.nil ty_unit :=
+    stm_write_register cur_privilege (exp_val ty_privilege Machine) ;;
     use lemma open_pmp_entries ;;
     call init_pmp ;;
-    use lemma close_pmp_entries.
+    use lemma update_pmp_entries.
 
   Definition fun_init_pmp : Stm ctx.nil ty_unit :=
     let: tmp := stm_read_register pmp0cfg in
